Annotated syntax defined and compiling

Total/Core.lean
@@ -23,15 +23,27 @@ section Functions
     | nil (ty: τ): Domain τ 1
     | cons {α: Nat} (ty: τ) (rest: Domain τ α): Domain τ α.succ
 
-  inductive Params {τ: Type}: {α: Nat} → Domain τ α → Type where
-    | nil (id: Nat) (ty: τ): Params (.nil ty)
-    | cons {α: Nat} {δ: Domain τ α} (id: ι) (ty: τ) (rest: Params δ): Params (.cons ty δ)
+  -- def Domain (τ: Type _): Type _ := Array τ
 
-  inductive Args {τ: Type} (t: τ → Type): {α: Nat} → Domain τ α → Type where
-    | nil {ty: τ} (arg: t ty): Args t (.nil ty)
-    | cons {α: Nat} {δ: Domain τ α} {ty: τ} (arg: t ty) (rest: Args t δ): Args t (.cons ty δ)
+  -- inductive Params {τ: Type}: {α: Nat} → Domain τ α → Type where
+  --   | nil (id: Nat) (ty: τ): Params (.nil ty)
+  --   | cons {α: Nat} {δ: Domain τ α} (id: ι) (ty: τ) (rest: Params δ): Params (.cons ty δ)
 
-  inductive Values {τ: Type} (t: τ → Type) (υ: {ty: τ} → t ty → Prop): {α: Nat} -> Domain τ α → Type where
-    | nil {ty: τ} {term: t ty} (v: υ term): Values t υ (.nil ty)
-    | cons {α: Nat} {δ: Domain τ α} {ty: τ} {term: t ty} (v: υ term) /- (rest: Values t υ δ) -/: Values t υ (.cons ty δ)
+  -- inductive Args {τ: Type} (t: τ → Type): {α: Nat} → Domain τ α → Type where
+  --   | nil {ty: τ} (arg: t ty): Args t (.nil ty)
+  --   | cons {α: Nat} {δ: Domain τ α} {ty: τ} (arg: t ty) (rest: Args t δ): Args t (.cons ty δ)
+
+  /-
+  Fails with:
+
+  (kernel) arg #9 of 'Values.cons' contains a non valid occurrence of the
+  datatypes being declared
+
+  I believe the issue is the parameter `υ`, since it has the `t ty` embedded in
+  it.  A type-specific version in the Grammar works fine.
+  -/
+  -- inductive Values {τ: Type _} {t: τ → Type _} (υ: {ty: τ} → t ty → Prop): {α: Nat} -> Domain τ α → Type _ where
+  --   | nil {ty: τ} {term: t ty} (v: υ term): Values υ (.nil ty)
+  --   | cons {α: Nat} {δ: Domain τ α} {ty: τ} {term: t ty} (v: υ term) (rest:
+  --   @Values τ t υ α δ): Values υ (.cons ty δ)
 end Functions
