Total/Stlc/Lang/Annotated/Grammar.lean
@@ -3,17 +3,29 @@ import Total.Core
 set_option autoImplicit false
 
 namespace Total.Stlc.Lang.Annotated
-  inductive Ty: Type where
-    | bool: Ty
-    | nat: Ty
-    | fn {α: Nat} (dom: Domain Ty α) (rng: Ty): Ty
+  mutual
+    inductive Ty: Type where
+      | bool: Ty
+      | nat: Ty
+      | fn {α: Nat} (dom: Domain α) (rng: Ty): Ty
 
-  abbrev Domain (α: Nat) := _root_.Domain Ty α
+    inductive Domain: Nat → Type where
+      | nil (τ: Ty): Domain 1
+      | cons {α: Nat} (τ: Ty) (rest: Domain α): Domain α.succ
+  end
+
+  instance: {α β: Nat} → HAppend (Domain α) (Domain β) (Domain (β + α)) where
+    hAppend lhs rhs :=
+      append lhs rhs
+      where
+        append {α β: Nat}: Domain α → Domain β → Domain (β + α)
+          | .nil τ, δ => .cons τ δ
+          | .cons τ rest, δ => .cons τ (append rest δ)
 
   inductive PrimOp: {α: Nat} → Domain α → Ty → Type where
     | and: PrimOp (.cons .bool (.nil .bool)) .bool
     | or:  PrimOp (.cons .bool (.nil .bool)) .bool
-    | not: PrimOp (.nil .bool) .bool
+    | not: PrimOp (.nil .nat)        .bool
 
     | add: PrimOp (.cons .nat (.nil .nat)) .nat
     | sub: PrimOp (.cons .nat (.nil .nat)) .nat
@@ -27,13 +39,29 @@ namespace Total.Stlc.Lang.Annotated
     | gt:  PrimOp (.cons .nat (.nil .nat)) .bool
     | gte: PrimOp (.cons .nat (.nil .nat)) .bool
 
-  inductive Term: Ty → Type where
-    | bool (b: Bool): Term .bool
-    | nat (n: Nat): Term .nat
-    | primOp {α: Nat} {δ: Domain α} {τ: Ty} (op: PrimOp δ τ) (operands: Args Term δ): Term (.fn δ τ)
-    | cond {τ: Ty} (c: Term .bool) (t f: Term τ): Term τ
+  mutual
+    inductive Value: Ty → Type where
+      | bool (b: Bool): Value .bool
+      | nat (n: Nat): Value .nat
 
-  abbrev Args {α: Nat} (δ: Domain α) := _root_.Args Term δ
+    inductive Values: {α: Nat} → Domain α → Type where
+      | nil {τ: Ty} (v: Value τ): Values (.nil τ)
+      | cons {τ: Ty} {α: Nat} {δ: Domain α} (v: Value τ) (rest: Values δ): Values (.cons τ δ)
+
+    inductive Term: Ty → Type where
+      | value {τ: Ty} (v: Value τ): Term τ
+      | primOp {α: Nat} {δ: Domain α} {τ: Ty}  (op: PrimOp δ τ) (operands: Args δ): Term (.fn δ τ)
+      | cond {τ: Ty} (c: Term .bool) (t f: Term τ): Term τ
+
+    inductive Terms: {α: Nat} → Domain α → Type where
+      | nil {τ: Ty} (t: Term τ): Terms (.nil τ)
+      | cons {τ: Ty} {α: Nat} {δ: Domain α} (t: Term τ) (rest: Terms δ): Terms (.cons τ δ)
+
+    inductive Args: {α: Nat} → Domain α → Type where
+      | terms {α: Nat} {δ: Domain α} (ts: Terms δ): Args δ
+      | mix {α β: Nat} {δ₁: Domain α} {δ₂: Domain β} (vs: Values δ₁) (ts: Terms δ₂): Args (δ₁ ++ δ₂)
+      | values {α: Nat} {δ: Domain α} (vs: Values δ): Args δ
+  end
 
   inductive Top: Ty → Type where
 end Total.Stlc.Lang.Annotated
